fix one more qnt_cnf issue (not enough rewriting)

src/HOL/SMT_Examples/SMT_Examples_Verit.thy
@@ -1122,35 +1122,40 @@ lemma
   using assms supply[[smt_trace]] by (smt (verit, ccfv_threshold)) (*qnt_cnf From: Galois_Energy_Games/Decidability.thy*)
 end
 
-abbreviation Deutsch_zero where "Deutsch_zero ≡ unit_vec 2 0"
-abbreviation Deutsch_one where "Deutsch_one ≡ unit_vec 2 1" 
-locale test =
+(*making it independent of complex_main, hence the redefinition of all types.*)
+locale test2 =
   fixes
-    one_mat :: "nat ⇒ 'complex_mat :: {plus,times}" (‹1⇩m›) and
-    smult_mat :: "'complex :: {plus,times,numeral,inverse,power} ⇒ 'complex_mat ⇒ 'complex_mat" (infixl ‹⋅⇩m› 70) and
-    ket_vec :: "'complex_vec ⇒ 'complex_mat" (‹|_⟩›) and
-    tensor_mat:: "['complex_mat, 'complex_mat] ⇒ 'complex_mat" (infixl ‹⨂› 63) and
-    dim_col :: "'complex_mat ⇒ nat"and
-    dim_row :: "'complex_mat ⇒ nat" and
-     QFT:: "nat ⇒ 'complex_mat"
+    one_mat :: "nat \<Rightarrow> 'complex_mat :: {plus,times,banach,real_normed_algebra_1}" (\<open>1\<^sub>m\<close>) and
+    smult_mat :: "'complex :: {plus,times,numeral,inverse,power} \<Rightarrow> 'complex_mat \<Rightarrow> 'complex_mat" (infixl \<open>\<cdot>\<^sub>m\<close> 70) and
+    ket_vec :: "'complex_vec \<Rightarrow> 'complex_mat" (\<open>|_\<rangle>\<close>) and
+    tensor_mat:: "['complex_mat, 'complex_mat] \<Rightarrow> 'complex_mat" (infixl \<open>\<Otimes>\<close> 63) and
+    dim_col :: "'complex_mat \<Rightarrow> nat"and
+    dim_row :: "'complex_mat \<Rightarrow> nat" and
+    QFT:: "nat \<Rightarrow> 'complex_mat" and
+    sqrt :: "'real \<Rightarrow> 'real::{times,numeral,inverse,one}" and
+    complex_of_real :: "'real \<Rightarrow> 'complex" and
+    complex_of_nat :: "nat \<Rightarrow> 'complex" and
+    imaginary_unit :: 'complex  (\<open>\<i>\<close>) and
+    pi :: 'real and
+    exp :: "'complex \<Rightarrow> 'complex"
 begin
 lemma
   assumes
-       "dim_col (1⇩m (2::nat)) =
-         dim_row (complex_of_real (1 / sqrt (2::'real)) ⋅⇩m (ket_vec Deutsch_zero + exp ((2::'complex) * 𝗂 * complex_of_real pi * complex_of_nat (j::nat) / (2::'complex) ^ Suc (n::nat)) ⋅⇩m |Deutsch_one⟩))"
-       "dim_col (QFT (n::nat)) = dim_row |state_basis n (jm::nat)⟩"
-       "0 < dim_col (1⇩m (2::nat))"
-       "0 < dim_col (complex_of_real (1 / sqrt (2::'real)) ⋅⇩m (ket_vec Deutsch_zero + exp ((2::'complex) * 𝗂 * complex_of_real pi * complex_of_nat (j::nat) / (2::'complex) ^ Suc (n::nat)) ⋅⇩m |Deutsch_one⟩))"
+       "dim_col (1\<^sub>m (2::nat)) =
+         dim_row (complex_of_real (1 / sqrt (2::'real)) \<cdot>\<^sub>m (ket_vec Deutsch_zero + exp ((2::'complex) * \<i> * complex_of_real pi * complex_of_nat (j::nat) / (2::'complex) ^ Suc (n::nat)) \<cdot>\<^sub>m |Deutsch_one\<rangle>))"
+       "dim_col (QFT (n::nat)) = dim_row |state_basis n (jm::nat)\<rangle>"
+       "0 < dim_col (1\<^sub>m (2::nat))"
+       "0 < dim_col (complex_of_real (1 / sqrt (2::'real)) \<cdot>\<^sub>m (ket_vec Deutsch_zero + exp ((2::'complex) * \<i> * complex_of_real pi * complex_of_nat (j::nat) / (2::'complex) ^ Suc (n::nat)) \<cdot>\<^sub>m |Deutsch_one\<rangle>))"
        "0 < dim_col (QFT (n::nat))"
-       "0 < dim_col |state_basis (n::nat) (jm::nat)⟩"
-       "∀(A::'complex_mat) (B::'complex_mat) (C::'complex_mat) D::'complex_mat.
-          dim_col A = dim_row B ∧ dim_col C = dim_row D ∧ 0 < dim_col A ∧ 0 < dim_col B ∧ 0 < dim_col C ∧ 0 < dim_col D ⟶ A * B ⨂ C * D = (A ⨂ C) * (B ⨂ D)"
-       "(1⇩m (2::nat) ⨂ QFT (n::nat)) *
-        (complex_of_real (1 / sqrt (2::'real)) ⋅⇩m (ket_vec Deutsch_zero + exp ((2::'complex) * 𝗂 * complex_of_real pi * complex_of_nat (j::nat) / (2::'complex) ^ Suc n) ⋅⇩m ket_vec Deutsch_one) ⨂
-        |state_basis n (jm::nat)⟩) ≠
-       1⇩m (2::nat) * (complex_of_real (1 / sqrt (2::'real::{numeral,plus,times})) ⋅⇩m (ket_vec Deutsch_zero + exp ((2::'complex) * 𝗂 * complex_of_real pi * complex_of_nat j / (2::'complex) ^ Suc n) ⋅⇩m ket_vec Deutsch_one)) ⨂
-       QFT n * |state_basis n jm⟩" 
+       "0 < dim_col |state_basis (n::nat) (jm::nat)\<rangle>"
+       "\<forall>(A::'complex_mat) (B::'complex_mat) (C::'complex_mat) D::'complex_mat.
+          dim_col A = dim_row B \<and> dim_col C = dim_row D \<and> 0 < dim_col A \<and> 0 < dim_col B \<and> 0 < dim_col C \<and> 0 < dim_col D \<longrightarrow> A * B \<Otimes> C * D = (A \<Otimes> C) * (B \<Otimes> D)"
+       "(1\<^sub>m (2::nat) \<Otimes> QFT (n::nat)) *
+        (complex_of_real (1 / sqrt (2::'real)) \<cdot>\<^sub>m (ket_vec Deutsch_zero + exp ((2::'complex) * \<i> * complex_of_real pi * complex_of_nat (j::nat) / (2::'complex) ^ Suc n) \<cdot>\<^sub>m ket_vec Deutsch_one) \<Otimes>
+        |state_basis n (jm::nat)\<rangle>) \<noteq>
+       1\<^sub>m (2::nat) * (complex_of_real (1 / sqrt (2::'real)) \<cdot>\<^sub>m (ket_vec Deutsch_zero + exp ((2::'complex) * \<i> * complex_of_real pi * complex_of_nat j / (2::'complex) ^ Suc n) \<cdot>\<^sub>m ket_vec Deutsch_one)) \<Otimes>
+       QFT n * |state_basis n jm\<rangle>" 
      shows False
-  using assms supply [[smt_trace,show_types]] apply (smt (verit, best))
+  using assms supply [[smt_trace=false,show_types]] by (smt (verit, best))
 end
 end
